Implement ReactionOutput.child (mod some Graph.Path properties)

Runtime/Network/Execution/ReactionOutput.lean
@@ -26,10 +26,11 @@ def Value.value? : Value α → Option α
   | present value        => value
   | independent | absent => none
 
--- Note: This theorem is really only needed for `Reaction.Output.local`.
+-- Note: This theorem is really only needed for `ReactionOutput.local`.
 private def local_type_correctness {output : ReactionOutput exec} {port port'} : 
   (output.reaction.portEffectsInjCoe.inv (.inl port) = some port') → 
-  (output.reactor.class.reactionOutputScheme |>.restrict output.reaction.portEffects |>.type port') = output.reactor.outputs.type port :=
+  (output.reactor.class.reactionOutputScheme |>.restrict output.reaction.portEffects |>.type port') = 
+  output.reactor.outputs.type port :=
   (by rw [Interface.Scheme.restrict_type, output.reaction.portEffectsInjCoe.invCoeId _ ·])
 
 def «local» (output : ReactionOutput exec) (port : output.reactor.outputs.vars) : Value (output.reactor.outputs.type port) := 
@@ -40,37 +41,20 @@ def «local» (output : ReactionOutput exec) (port : output.reactor.outputs.vars
     | none => .absent
     | some value => .present (local_type_correctness h ▸ value)
 
-def child (output : ReactionOutput exec) {child : ReactorId.Child output.reactor} (port : (child : ReactorId net).inputs.vars) : Value ((child : ReactorId net).inputs.type port) := 
-  -- match h : output.reaction.portEffectsInjCoe.inv (.inr ⟨child.class, port⟩) with
-  -- | none => .independent
-  -- | some port' =>
-  --   match output.raw.ports port' with
-  --   | none => .absent
-  --   | some value => .present (local_type_correctness h ▸ value)
-  sorry
-    -- nestedInputs (exec : Executable net) (output : Reaction.Output net) (id : ReactorId net) (hc : id ≻ output.reactor) : Interface? (id.class.interface .inputs) :=
-  --  let currentReactor := exec.reactors id
-  --  fun var =>
-      /-
-      let nestedID := id.last hc
-      have h₁ : (net.scheme id |>.interface .inputs).vars = (net.subinterface (net.class reactorID) nestedID .inputs).vars := by sorry -- rw [Graph.child_schemes_eq_parent_subschemes]
-      let var₁ : (net.reactionOutputScheme' reactorID).vars := .inr ⟨nestedID, h₁ ▸ var⟩
-      match h : InjectiveCoe.inv var₁ with 
-      | none => currentReactor.interface .inputs var
-      | some var₂ =>
-        match output.ports var₂ with
-        | none => currentReactor.interface .inputs var
-        | some val =>
-          have h : (net.class reactorID |> net.reactionOutputScheme |>.restrict reaction.portEffects).type var₂ = (net.scheme id |>.interface .inputs).type var := by
-            rw [(net.reactionOutputScheme' reactorID).restrict_type]
-            rw [InjectiveCoe.invCoeId _ h]
-            -- have := Graph.child_schemes_eq_parent_subschemes hc
-            sorry
-          h ▸ val
-      -/
+-- Note: This theorem is really only needed for `ReactionOutput.child`.
+private def child_type_correctness {output : ReactionOutput exec} {child : ReactorId.Child output.reactor} {port port'} : 
+  (output.reaction.portEffectsInjCoe.inv (.inr ⟨child.class, port⟩) = some port') →
+  ((output.reactor.class.reactionOutputScheme).restrict output.reaction.portEffects).type port' =
+  (child.class.class.interface .inputs).type port :=
+  (by rw [Interface.Scheme.restrict_type, output.reaction.portEffectsInjCoe.invCoeId _ ·]; rfl)
 
-
-
+def child (output : ReactionOutput exec) {child : ReactorId.Child output.reactor} (port : child.class.class.interface .inputs |>.vars) : Value (child.class.class.interface .inputs |>.type port) := 
+  match h : output.reaction.portEffectsInjCoe.inv (.inr ⟨child.class, port⟩) with
+  | none => .independent
+  | some port' =>
+    match output.raw.ports port' with
+    | none => .absent
+    | some value => .present (child_type_correctness h ▸ value)
 
 theorem events_LawfulQueue (output : ReactionOutput exec) : Executable.LawfulQueue output.events exec.tag.time := by
   intro _ h
